Factor out ConsExp into new module

Fine/PropositionalLanguage.lean
@@ -1,6 +1,6 @@
 import Mathlib.Init.Set
 import Mathlib.Logic.Denumerable
-import Mathlib.Data.Finite.Defs
+import Fine.Util.ConsExp
 
 inductive Form : Type
   | atom : Nat → Form
@@ -16,74 +16,6 @@ infixr:512 "&" => Form.and
 infixr:512 "¦" => Form.or
 prefix:max "~" => Form.neg
 
-inductive ConsExp : Type
-  | nat : Nat → ConsExp
-  | cons : ConsExp → ConsExp → ConsExp
-
-def ConsExp.encode : ConsExp → Nat
-  | nat n => 2 * n
-  | cons f g => 2 * Nat.mkpair f.encode g.encode + 1
-
-def ConsExp.decode (n : ℕ) : ConsExp :=
-  match hn : Nat.boddDiv2 n with
-  | (false, m) => nat m
-  | (true, m) =>
-    match hm : Nat.unpair m with
-    | (f, g) =>
-      -- Some proofs to show termination:
-      have hn' : 1 ≤ n := by
-        cases n
-        · simp at hn
-        · simp [Nat.succ_eq_add_one]
-      have : m < n := by
-        have := congr_arg Prod.snd hn
-        simp at this
-        cases this
-        apply Nat.binaryRec_decreasing
-        rwa [Nat.one_le_iff_ne_zero] at hn'
-      have : f < n := by
-        apply Nat.lt_of_le_of_lt _ this
-        have := congr_arg Prod.fst hm
-        simp at this
-        cases this
-        cases m
-        · simp
-        next m =>
-          apply (Nat.unpair_lt _).le
-          simp [Nat.succ_eq_add_one]
-      have : g < n := by
-        have := congr_arg Prod.snd hm
-        simp at this
-        cases this
-        have := Nat.unpair_right_le m
-        apply Nat.lt_of_le_of_lt this
-        assumption
-      -- With those out of the way:
-      cons (decode f) (decode g)
-termination_by _ => n
-
-theorem ConsExp.decode_encode (c : ConsExp) : ConsExp.decode c.encode = c := by
-  induction c
-  · rw [encode, decode]
-    split
-    next h =>
-      simp [Nat.div2_val] at h
-      simp [*]
-    next h => simp at h
-  next hf hg =>
-    rw [encode, decode]
-    split
-    next h => simp at h
-    next h =>
-      simp [Nat.div2_val] at h
-      cases h
-      simp [*]
-
-instance : Encodable ConsExp where
-  encode := ConsExp.encode
-  decode := fun v => some (ConsExp.decode v)
-  encodek := fun a => by simp [ConsExp.decode_encode]
-
 def Form.toConsExp : Form → ConsExp
   | atom n => .cons (.nat 0) (.nat n)
   | neg f => .cons (.nat 1) f.toConsExp
@@ -94,6 +26,11 @@ def Form.toConsExp : Form → ConsExp
 theorem Form.toConsExp_injective : Function.Injective Form.toConsExp := by
   intros f1 f2
   induction f1 generalizing f2 <;> cases f2 <;> simp! <;> aesop
+
+theorem Form.nat_injection : Function.Injective Form.atom := by
+  unfold Function.Injective;
+  intros n m h₁
+  injection h₁
 
 def ConsExp.toForm : ConsExp → Option Form
   | .cons (.nat 0) (.nat n) => .some (.atom n)
@@ -106,12 +43,17 @@ def ConsExp.toForm : ConsExp → Option Form
 theorem toForm_toConsExp_eq (f : Form) : f.toConsExp.toForm = some f := by
   induction f <;> simp! [*]
 
+instance Form.infinite : Infinite Form := 
+  Infinite.of_injective Form.atom Form.nat_injection
+
 instance : Encodable Form where
   encode f := Encodable.encode f.toConsExp
   decode n := Option.bind (Encodable.decode n) ConsExp.toForm 
   encodek := by
     intro f
     simp [toForm_toConsExp_eq]
+
+instance : Denumerable Form := Denumerable.ofEncodableOfInfinite Form
     
 instance : ToString Form where
   toString := display
