Fine/Util/ConsExp.lean
@@ -1,0 +1,69 @@
+import Mathlib.Logic.Denumerable
+
+inductive ConsExp : Type
+  | nat : Nat → ConsExp
+  | cons : ConsExp → ConsExp → ConsExp
+
+def ConsExp.encode : ConsExp → Nat
+  | nat n => 2 * n
+  | cons f g => 2 * Nat.mkpair f.encode g.encode + 1
+
+def ConsExp.decode (n : ℕ) : ConsExp :=
+  match hn : Nat.boddDiv2 n with
+  | (false, m) => nat m
+  | (true, m) =>
+    match hm : Nat.unpair m with
+    | (f, g) =>
+      -- Some proofs to show termination:
+      have hn' : 1 ≤ n := by
+        cases n
+        · simp at hn
+        · simp [Nat.succ_eq_add_one]
+      have : m < n := by
+        have := congr_arg Prod.snd hn
+        simp at this
+        cases this
+        apply Nat.binaryRec_decreasing
+        rwa [Nat.one_le_iff_ne_zero] at hn'
+      have : f < n := by
+        apply Nat.lt_of_le_of_lt _ this
+        have := congr_arg Prod.fst hm
+        simp at this
+        cases this
+        cases m
+        · simp
+        next m =>
+          apply (Nat.unpair_lt _).le
+          simp [Nat.succ_eq_add_one]
+      have : g < n := by
+        have := congr_arg Prod.snd hm
+        simp at this
+        cases this
+        have := Nat.unpair_right_le m
+        apply Nat.lt_of_le_of_lt this
+        assumption
+      -- With those out of the way:
+      cons (decode f) (decode g)
+termination_by _ => n
+
+theorem ConsExp.decode_encode (c : ConsExp) : ConsExp.decode c.encode = c := by
+  induction c
+  · rw [encode, decode]
+    split
+    next h =>
+      simp [Nat.div2_val] at h
+      simp [*]
+    next h => simp at h
+  next hf hg =>
+    rw [encode, decode]
+    split
+    next h => simp at h
+    next h =>
+      simp [Nat.div2_val] at h
+      cases h
+      simp [*]
+
+instance : Encodable ConsExp where
+  encode := ConsExp.encode
+  decode := fun v => some (ConsExp.decode v)
+  encodek := fun a => by simp [ConsExp.decode_encode]
